aaaaaaaaaaaa

src/fopl_ar.lean
@@ -10,6 +10,8 @@ structure language : Type (u+1) :=
 (fn : ℕ → Type u)
 (pr : ℕ → Type u)
 
+class has_eq_symbol (L : language) := (eq : L.pr 2)
+
 class has_zero_symbol (L : language) := (zero : L.fn 0)
 
 class has_succ_symbol (L : language) := (succ : L.fn 1)
@@ -64,12 +66,13 @@ instance [∀ n, has_to_string (L.fn n)] {β} : has_to_string (term L β) := ⟨
 inductive formula : ℕ → Type u
 | verum : Π {β}, formula β
 | app   : ∀ {β n : ℕ}, L.pr n → (fin n → term L β) → formula β
-| equal : ∀ {β}, term L β → term L β → formula β
 | imply : ∀ {β}, formula β → formula β → formula β
 | neg   : ∀ {β}, formula β → formula β
 | fal   : ∀ {β}, formula (β + 1) → formula β
 
 notation `❴` c `❵` := formula.app c
+
+instance [has_eq_symbol L] {β} : has_eq (term L β) (formula L β) := ⟨λ t u, formula.app has_eq_symbol.eq ‹t, u›⟩
 
 instance [has_le_symbol L] {β} : has_preceq (term L β) (formula L β) := ⟨λ t u, formula.app has_le_symbol.le ‹t, u›⟩
 
@@ -81,15 +84,9 @@ instance : has_top (formula L β) := ⟨formula.verum⟩
 
 instance : has_arrow (formula L β) := ⟨formula.imply⟩
 
-instance : has_eq (term L β) (formula L β) := ⟨formula.equal⟩
-
-local infix ` ≃₁ `:80 := ((≃) : term L β → term L β → formula L β)
-
 instance {β} : has_negation (formula L β) := ⟨formula.neg⟩
 
 instance : has_univ_quantifier' (formula L) := ⟨λ β, formula.fal⟩
-
-prefix `ℿ`:64 := formula.fal
 
 instance {β} : has_bot (formula L β) := ⟨⁻⊤⟩
 
@@ -102,7 +99,6 @@ def formula_to_string [∀ β, has_to_string (term L β)] [∀ n, has_to_string 
     has_to_string.to_string (v 0) ++ has_to_string.to_string p ++ has_to_string.to_string (v 1)
 | β (@formula.app _ _ (n + 3) p v) :=
     has_to_string.to_string p ++ "(" ++ @has_to_string.to_string (finitary _ _) _ v ++ ")"
-| β (formula.equal t u)            := has_to_string.to_string t ++ " = " ++ has_to_string.to_string u
 | β (formula.imply p q)            := formula_to_string p ++ " → " ++ formula_to_string q
 | β (formula.neg p)                := "¬(" ++ formula_to_string p ++ ")"
 | β (formula.fal p)                := "∀(" ++ formula_to_string p ++ ")"
@@ -112,13 +108,10 @@ instance [∀ β, has_to_string (term L β)] [∀ n, has_to_string (L.pr n)] : h
 
 @[simp] lemma formula.top_eq : @formula.verum L = (⊤) := rfl
 @[simp] lemma formula.imply_eq : @formula.imply L β = (⟶) := rfl
-@[simp] lemma formula.equal_eq : @formula.equal L β = (≃) := rfl
 @[simp] lemma formula.neg_eq : @formula.neg L β = has_negation.neg := rfl
 @[simp] lemma formula.fal_eq : @formula.fal L β = has_univ_quantifier'.univ := rfl
 
 instance : inhabited (formula L β) := ⟨⊤⟩
-
-@[reducible] def theory (L : language.{u}) (β) := set (formula L β)
 
 variables {L} {β} {γ : ℕ}
 
@@ -135,9 +128,6 @@ def formula.ex (p : formula L (β + 1)) : formula L β := ⁻𝚷⁻p
 instance : has_exists_quantifier' (formula L) := ⟨λ _, formula.ex⟩
 
 lemma formula.ex_eq (p : formula L (β + 1)) : (𝚺 p : formula L β) = ⁻𝚷⁻p := rfl
-
-@[simp] lemma formula.equal.inj' (t₁ u₁ t₂ u₂ : term L β) : (t₁ ≃ t₂ : formula L β) = (u₁ ≃ u₂) ↔ t₁ = u₁ ∧ t₂ = u₂ :=
-⟨formula.equal.inj, by simp; exact congr_arg2 (≃)⟩
 
 @[simp] lemma formula.imply.inj' (p₁ q₁ p₂ q₂ : formula L β) : p₁ ⟶ p₂ = q₁ ⟶ q₂ ↔ p₁ = q₁ ∧ p₂ = q₂ :=
 ⟨formula.imply.inj, by simp; exact congr_arg2 (⟶)⟩
@@ -158,8 +148,6 @@ by simp[has_exists_quantifier'.ex, formula.ex]
 @[simp] lemma formula.verum_ne_predicate {n} (r : L.pr n) (v : finitary (term L β) n) :
  ⊤ ≠ formula.app r v.
 
-@[simp] lemma formula.verum_ne_equal (t u : term L β) : (⊤ : formula L β) ≠ (t ≃ u).
-
 @[simp] lemma formula.verum_ne_imply (p q : formula L β) : ⊤ ≠ (p ⟶ q).
 
 @[simp] lemma formula.verum_ne_neg (p : formula L β) : ⊤ ≠ ⁻p.
@@ -168,9 +156,6 @@ by simp[has_exists_quantifier'.ex, formula.ex]
 
 @[simp] lemma formula.predicate_ne_verum {n} (r : L.pr n) (v : finitary (term L β) n) :
   formula.app r v ≠ ⊤.
-
-@[simp] lemma formula.predicate_ne_equal {n} (r : L.pr n) (v : finitary (term L β) n) (t u : term L β) :
-  formula.app r v ≠ (t ≃ u).
 
 @[simp] lemma formula.predicate_ne_imply {n} (r : L.pr n) (v : finitary (term L β) n) (p q : formula L β) :
   formula.app r v ≠ p ⟶ q.
@@ -181,29 +166,11 @@ by simp[has_exists_quantifier'.ex, formula.ex]
 @[simp] lemma formula.predicate_ne_fal {n} (r : L.pr n) (v : finitary (term L β) n) (p) :
   formula.app r v ≠ 𝚷 p.
 
-@[simp] lemma formula.equal_ne_verum (t u : term L β) :
-  (t ≃ u : formula L β) ≠ ⊤.
-
-@[simp] lemma formula.equal_ne_predivate (t u : term L β) {n} (r : L.pr n) (v : finitary (term L β) n) :
-  (t ≃ u) ≠ formula.app r v.
-
-@[simp] lemma formula.equal_ne_imply (t u : term L β) (p q : formula L β) :
-  (t ≃ u) ≠ p ⟶ q.
-
-@[simp] lemma formula.equal_ne_neg (t u : term L β) (p : formula L β) :
-  (t ≃ u) ≠ ⁻p.
-
-@[simp] lemma formula.equal_ne_fal (t u : term L β) (p) :
-  (t ≃ u : formula L β) ≠ 𝚷 p.
-
 @[simp] lemma formula.imply_ne_verum (p q : formula L β) :
   p ⟶ q ≠ ⊤.
 
 @[simp] lemma formula.imply_ne_predicate (p q : formula L β) {n} (r : L.pr n) (v : finitary (term L β) n) :
   p ⟶ q ≠ formula.app r v.
-
-@[simp] lemma formula.imply_ne_equal (p q : formula L β) (t u : term L β) :
-  p ⟶ q ≠ (t ≃ u).
 
 @[simp] lemma formula.imply_ne_neg (p q r : formula L β) : p ⟶ q ≠ ⁻r.
 
@@ -214,8 +181,6 @@ by simp[has_exists_quantifier'.ex, formula.ex]
 @[simp] lemma formula.neg_ne_predicate (p : formula L β) {n} (r : L.pr n) (v : finitary (term L β) n) :
  ⁻p ≠ formula.app r v.
 
-@[simp] lemma formula.neg_ne_equal (p : formula L β) (t u : term L β) : ⁻p ≠ (t ≃ u).
-
 @[simp] lemma formula.neg_ne_imply (p q r : formula L β) : ⁻p ≠ (q ⟶ r).
 
 @[simp] lemma formula.neg_ne_fal (p : formula L β) (q) : ⁻p ≠ 𝚷 q.
@@ -225,9 +190,6 @@ by simp[has_exists_quantifier'.ex, formula.ex]
 
 @[simp] lemma formula.fal_ne_predicate (p : formula L (β + 1)) {n} (r : L.pr n) (v : finitary (term L β) n) :
   𝚷 p ≠ formula.app r v.
-
-@[simp] lemma formula.fal_ne_equal (p : formula L (β + 1)) (t u : term L β) :
-  (𝚷 p : formula L β) ≠ (t ≃ u).
 
 @[simp] lemma formula.fal_ne_imp (p : formula L (β + 1)) (q r : formula L β) : 𝚷 p ≠ (q ⟶ r).
 
@@ -273,6 +235,8 @@ namespace term
 | β γ s (#x)           := s x
 | β γ s (term.app f v) := ❨f❩ (λ i, rew s (v i))
 
+@[reducible] def rew_var (s : fin β → fin γ) : term L β → term L γ := λ t, t.rew (λ x, #(s x))
+
 @[simp] lemma nested_rew : ∀ {β γ δ} (t : term L β) (s₀ : finitary (term L γ) β) (s₁ : finitary (term L δ) γ),
   (t.rew s₀).rew s₁ = t.rew (λ x, (s₀ x).rew s₁)
 | β γ δ (#x)     := by simp[rew]
@@ -288,7 +252,10 @@ instance : has_shift (term L) := ⟨@shift L⟩
 lemma shift_eq (t : term L β) : ⤉t = t.rew (λ i, #(i + 1)) := rfl
 
 lemma pow_eq (t : term L β) (k) : t ↟ k = t.rew (λ x, #(⟨x + k, by simp⟩)) :=
-by { induction k with k IH; simp[*, shift_eq, nested_rew , ←nat.add_one, add_assoc], refl }
+by { induction k with k IH; simp[*, has_shift.shifts_succ, shift_eq, nested_rew, ←nat.add_one, add_assoc], refl }
+
+lemma pow_eq_rew_var (t : term L β) (k) : t ↟ k = t.rew_var (λ x, ⟨x + k, by simp⟩) :=
+by simp[pow_eq]
 
 def lift : Π {β}, term L β → term L (β + 1) := λ β t, t.rew (λ i, #i)
 
@@ -303,8 +270,6 @@ instance : has_shift' (term L) := ⟨@lift L⟩
 
 @[simp] lemma lift_function {n} (f : L.fn n) (v : finitary (term L β) n) :
   ⤉'(term.app f v : term L β) = term.app f (λ i, ⤉'(v i)) := by simp[has_shift'.shift', lift]
-
-@[reducible] def rew_var (s : fin β → fin γ) : term L β → term L γ := λ t, t.rew (λ x, #(s x))
 
 @[simp] lemma constant_rew (c : L.fn 0) (s : finitary (term L γ) β) {v : finitary (term L β) 0} :
   (app c v : term L β).rew s = app c finitary.nil :=
@@ -338,11 +303,11 @@ by unfold has_add.add; simp; ext; simp
 by unfold has_mul.mul; simp; ext; simp
 
 @[simp] lemma var_pow (n : fin β) (k : ℕ) : (#n : term L β) ↟ k = #⟨n + k, by simp⟩ :=
-by induction k with k IH; simp[*, ←nat.add_one, add_assoc]
+by induction k with k IH; simp[*, has_shift.shifts_succ, ←nat.add_one, add_assoc]
 
 @[simp] lemma app_pow {n} (f : L.fn n) (v : finitary' (term L) n β) (k : ℕ) :
   (❨f❩ v) ↟ k = ❨f❩ (v ↟ k) :=
-by {induction k with k IH; simp*, funext i, simp }
+by {induction k with k IH; simp[*, has_shift.shifts_succ], funext i, simp }
 
 @[simp] lemma app_lift_pow {n} (f : L.fn n) (v : finitary' (term L) n β) (k : ℕ) :
   (❨f❩ v) ↟' k = ❨f❩ (v ↟' k) :=
@@ -376,7 +341,7 @@ by unfold has_add.add; simp
 @[simp] lemma mul_pow [h : has_mul_symbol L] (t u : term L β) (k : ℕ) : (t * u : term L β) ↟ k = t ↟ k * u ↟ k :=
 by unfold has_mul.mul; simp
 
-@[simp] lemma rew_var_inj_of_inj :
+lemma rew_var_inj_of_inj :
   ∀ {β} {t u : term L β} {s : fin β → fin γ} (I : function.injective s),
   t.rew_var s = u.rew_var s ↔ t = u
 | β #x               #y               s I := by { simp[rew_var], exact ⟨@I x y, congr_arg (λ x, s x)⟩ }
@@ -392,20 +357,8 @@ by unfold has_mul.mul; simp
       { rintros rfl, simp }
     end
 
-@[simp] lemma pow_inj :
-  ∀ {β} {t u : term L β} {k : ℕ}, t ↟ k = u ↟ k ↔ t = u
-| β #x               #y               k := by { simp, exact set_coe.ext_iff }
-| β #x               (term.app f v)   k := by simp
-| β (term.app f v)   #x               k := by simp
-| β (term.app f₁ v₁) (term.app f₂ v₂) k :=
-    begin
-      simp, rintros rfl, simp, intros, split,
-      { intros h, funext i,
-        have : (v₁ i) ↟ k = (v₂ i) ↟ k,
-        { have := congr_fun h i, simp at this, exact this },
-        exact (@pow_inj β (v₁ i) (v₂ i) k).mp this },
-      { rintros rfl, simp }
-    end
+@[simp] lemma pow_inj {β} {t u : term L β} {k : ℕ} : t ↟ k = u ↟ k ↔ t = u :=
+by { simp[pow_eq_rew_var], refine rew_var_inj_of_inj (λ x y, by { simp, exact fin.ext }) }
 
 @[simp] lemma finitary_pow_inj {n} {v w : finitary' (term L) n β} {i : ℕ} : v ↟ i = w ↟ i ↔ v = w :=
 ⟨λ h, funext (λ i, by { have := congr_fun h i, simp at this, exact this }),
@@ -437,12 +390,11 @@ by { simp[rewsf], ext ⟨i, h⟩, cases i; simp }
 namespace formula
 
 @[simp] def rew : Π {β γ}, (finitary (term L γ) β) → formula L β → formula L γ
-| β γ s formula.verum         := ⊤
-| β γ s (app p v) := app p (λ i, (v i).rew s)
-| β γ s (formula.equal t u)  := (t.rew s) ≃ (u.rew s)
-| β γ s (formula.imply p q)  := p.rew s ⟶ q.rew s
-| β γ s (formula.neg p)      := ⁻(p.rew s)
-| β γ s (formula.fal p)      := 𝚷 (rew (rewsf s) p)
+| β γ s formula.verum       := ⊤
+| β γ s (app p v)           := app p (λ i, (v i).rew s)
+| β γ s (formula.imply p q) := p.rew s ⟶ q.rew s
+| β γ s (formula.neg p)     := ⁻(p.rew s)
+| β γ s (formula.fal p)     := 𝚷 (rew (rewsf s) p)
 
 @[reducible] def rew_var (s : fin β → fin γ) : formula L β → formula L γ := λ p, p.rew (λ x, #(s x))
 
@@ -457,6 +409,10 @@ by simp; ext; simp
   (❴p❵ v).rew s = ❴p❵ ‹(v 0).rew s, (v 1).rew s› :=
 by simp; ext; simp
 
+@[simp] lemma eq_rew [c : has_eq_symbol L] (t u : term L β) (s : finitary (term L γ) β) :
+  (t ≃ u : formula L β).rew s = (t.rew s ≃ u.rew s) :=
+by unfold has_eq.eq; simp
+
 @[simp] lemma le_rew [c : has_le_symbol L] (t u : term L β) (s : finitary (term L γ) β) :
   (t ≼ u : formula L β).rew s = (t.rew s ≼ u.rew s) :=
 by unfold has_preceq.preceq; simp
@@ -465,20 +421,24 @@ by unfold has_preceq.preceq; simp
   (t ∊ u : formula L β).rew s = (t.rew s ∊ u.rew s) :=
 by unfold has_elem.elem; simp
 
-@[simp] lemma equal_rew (t u : term L β) (s : finitary (term L γ) β) :
-  (t ≃ u : formula L β).rew s = (t.rew s ≃ u.rew s) := rfl
 @[simp] lemma verum_rew (s : finitary (term L γ) β) :
   (⊤ : formula L β).rew s = ⊤ := rfl
+
 @[simp] lemma neg_rew (p : formula L β) (s : finitary (term L γ) β) :
   (⁻p).rew s = ⁻(p.rew s) := rfl
+
 @[simp] lemma imply_rew (p q : formula L β) (s : finitary (term L γ) β) :
   (p ⟶ q).rew s = p.rew s ⟶ q.rew s := rfl
+
 @[simp] lemma fal_rew (p : formula L (β + 1)) (s : finitary (term L γ) β) :
   (𝚷 p).rew s = 𝚷 (rew (rewsf s) p) := rfl
+
 @[simp] lemma and_rew (p q : formula L β) (s : finitary (term L γ) β) :
   (p ⊓ q).rew s = p.rew s ⊓ q.rew s := rfl
+
 @[simp] lemma or_rew (p q : formula L β) (s : finitary (term L γ) β) :
   (p ⊔ q).rew s = p.rew s ⊔ q.rew s := rfl
+
 @[simp] lemma iff_rew (p q : formula L β) (s : finitary (term L γ) β) :
   (p ⟷ q).rew s = p.rew s ⟷ q.rew s := rfl
 
@@ -504,11 +464,10 @@ by { induction n with n IH; simp* }
 
 lemma nested_rew : ∀ {β γ δ} (p : formula L β) (s₀ : finitary (term L γ) β) (s₁ : finitary (term L δ) γ),
   (p.rew s₀).rew s₁ = p.rew (λ x, (s₀ x).rew s₁)
-| β γ δ formula.verum         _ _ := by simp
-| β γ δ (❴p❵ v) _ _ := by simp[rew]
-| β γ δ (formula.equal t u)  _ _ := by simp[rew]
-| β γ δ (formula.imply p q)   _ _ := by simp[rew, nested_rew p, nested_rew q]
-| β γ δ (formula.neg p)      _ _ := by simp[rew]; refine nested_rew p _ _
+| β γ δ formula.verum       _ _ := by simp
+| β γ δ (❴p❵ v)             _ _ := by simp[rew]
+| β γ δ (formula.imply p q) _ _ := by simp[rew, nested_rew p, nested_rew q]
+| β γ δ (formula.neg p)     _ _ := by simp[rew]; refine nested_rew p _ _
 | β γ δ (formula.fal p)     _ _ := by { simp[rew, nested_rew p], congr,
     ext ⟨n, h⟩, cases n; simp[rewsf, term.shift_eq] }
 
@@ -519,7 +478,7 @@ instance : has_shift (formula L) := ⟨@shift L⟩
 lemma shift_eq (p : formula L β) : ⤉p = p.rew (λ x, #x.succ) := rfl
 
 lemma pow_eq (p : formula L β) (k) : p ↟ k = p.rew (λ x, #(⟨x + k, by simp⟩)) :=
-by { induction k with k IH; simp[*, shift_eq, nested_rew , ←nat.add_one, add_assoc], refl }
+by { induction k with k IH; simp[*, has_shift.shifts_succ, shift_eq, nested_rew , ←nat.add_one, add_assoc], refl }
 
 lemma pow_eq_rew_var (p : formula L β) (k) : p ↟ k = p.rew_var (λ x, ⟨x + k, by simp⟩) :=
 by simp[pow_eq]
@@ -529,14 +488,18 @@ by simp[pow_eq]
 
 @[simp] lemma constant_pow (c : L.pr 0) (k : ℕ) {v : finitary (term L β) 0} :
   (app c v) ↟ k = app c finitary.nil :=
-by induction k; simp*
+by induction k; simp[*, has_shift.shifts_succ]
 
 @[simp] lemma unary_pow (p : L.pr 1) (k : ℕ) (t : term L β) : (❴p❵ ‹t›) ↟ k = ❴p❵ ‹t ↟ k› :=
-by induction k with k IH; simp*
+by induction k with k IH; simp[*, has_shift.shifts_succ]
 
 @[simp] lemma binary_pow (p : L.pr 2) (k : ℕ) (t₁ t₂ : term L β) :
   (❴p❵ ‹t₁, t₂›) ↟ k = ❴p❵ ‹t₁ ↟ k, t₂ ↟ k› :=
-by induction k with k IH; simp*
+by induction k with k IH; simp[*, has_shift.shifts_succ]
+
+@[simp] lemma eq_pow [c : has_eq_symbol L] (t u : term L β) (k : ℕ) :
+  (t ≃ u : formula L β) ↟ k = (t ↟ k ≃ u ↟ k) :=
+by unfold has_eq.eq; induction k with k IH; simp*
 
 @[simp] lemma le_pow [c : has_le_symbol L] (t u : term L β) (k : ℕ) :
   (t ≼ u : formula L β) ↟ k = (t ↟ k ≼ u ↟ k) :=
@@ -546,7 +509,6 @@ by unfold has_preceq.preceq; induction k with k IH; simp*
   (t ∊ u : formula L β) ↟ k = (t ↟ k ∊ u ↟ k) :=
 by unfold has_elem.elem; induction k with k IH; simp*
 
-@[simp] lemma eq_pow (t u : term L β) (k : ℕ) : (t ≃₁ u) ↟ k = (t ↟ k ≃ u ↟ k) := by simp[term.pow_eq, pow_eq]
 @[simp] lemma imply_pow (p q : formula L β) (k : ℕ) : (p ⟶ q) ↟ k = p ↟ k ⟶ q ↟ k := by simp[pow_eq]
 @[simp] lemma neg_pow (p : formula L β) (k : ℕ) : (⁻p) ↟ k = ⁻(p ↟ k) := by simp[pow_eq]
 @[simp] lemma and_pow (p q : formula L β) (k : ℕ) : (p ⊓ q) ↟ k = (p ↟ k) ⊓ (q ↟ k) := by simp[pow_eq]
@@ -554,14 +516,16 @@ by unfold has_elem.elem; induction k with k IH; simp*
 @[simp] lemma top_pow (k : ℕ) : (⊤ : formula L β) ↟ k = ⊤ := by simp[pow_eq]
 @[simp] lemma bot_pow (k : ℕ) : (⊥ : formula L β) ↟ k = ⊥ := by simp[pow_eq]
 
-lemma fal_shift_discard (p : formula L (β + 1)) : ⤉(𝚷 p) = 𝚷 (p.rew (rewsf (λ x, #x.succ))) :=
+lemma fal_shift_discard (p : formula L (β + 1)) :
+  ⤉(𝚷 p) = 𝚷 (p.rew (rewsf (λ x, #x.succ))) :=
 by simp[shift_eq]
 
 lemma fal_pow (p : formula L (β + 1)) (k : ℕ) :
   (𝚷 p) ↟ k = 𝚷 (p.rew (rewsf (λ x, #(⟨x + k, by simp⟩ : fin (β + k))))) :=
 by simp[pow_eq]
 
-lemma ex_shift_discard (p : formula L (β + 1)) : ⤉(𝚺 p) = 𝚺 (p.rew (rewsf (λ x, #x.succ))) :=
+lemma ex_shift_discard (p : formula L (β + 1)) :
+  ⤉(𝚺 p) = 𝚺 (p.rew (rewsf (λ x, #x.succ))) :=
 by simp[shift_eq]
 
 lemma ex_pow (p : formula L (β + 1)) (k : ℕ) :
@@ -581,7 +545,7 @@ by { suffices : p.rew s = p.rew ι, { simp at this, exact this }, refine rew_rew
 lemma pow_rew_distrib  (p : formula L β) (s : finitary' (term L) β γ) (k : ℕ) :
   (p.rew s) ↟ k = (p ↟ k).rew (rewsf_itr s k) :=
 by { induction k with k IH generalizong s, { simp },
-     { simp[←nat.add_one, nested_rew, IH, shift_eq],
+     { simp[has_shift.shifts_succ, ←nat.add_one, nested_rew, IH, shift_eq],
        refine rew_rew _ (funext (λ i, _)), simp[rewsf, term.shift_eq] } }
 
 lemma rewriting_sf_perm {s : finitary (term L γ) β} (h : ∀ n, ∃ m, s m = #n) : ∀ n, ∃ m, (rewsf s) m = #n :=
@@ -592,17 +556,14 @@ lemma rewriting_sf_perm {s : finitary (term L γ) β} (h : ∀ n, ∃ m, s m = #
 lemma total_rew_inv :
   ∀ {β} {γ} (s : finitary (term L γ) β) (h : ∀ n, ∃ m, s m = #n) (p : formula L γ), ∃ q : formula L β, q.rew s = p
 | β γ _ _ formula.verum := ⟨⊤, by simp⟩
-| β γ s h (@app _ _ n p v) :=
+| β γ s h (@app _ _ n p v)    :=
     by rcases classical.skolem.mp (λ i : fin n, @term.total_rew_inv _ β γ s h (v i : term L γ)) with ⟨w, w_p⟩;
     refine ⟨❴p❵ w, by simp[w_p]⟩
-| β γ s h (formula.equal t u)       := 
-    by rcases term.total_rew_inv s h t with ⟨w₁, e_w₁⟩;
-       rcases term.total_rew_inv s h u with ⟨w₂, e_w₂⟩; refine ⟨w₁ ≃ w₂, by simp[e_w₁, e_w₂]⟩
-| β γ s h (formula.imply p q)        := 
+| β γ s h (formula.imply p q) := 
     by rcases total_rew_inv s h p with ⟨p', e_p'⟩;
        rcases total_rew_inv s h q with ⟨q', e_q'⟩; refine ⟨p' ⟶ q', by simp*⟩
-| β γ s h (formula.neg p)           := by rcases total_rew_inv s h p with ⟨q, e_q⟩; refine ⟨⁻q, by simp*⟩
-| β γ s h (formula.fal p)          :=
+| β γ s h (formula.neg p)     := by rcases total_rew_inv s h p with ⟨q, e_q⟩; refine ⟨⁻q, by simp*⟩
+| β γ s h (formula.fal p)     :=
   by rcases total_rew_inv _ (rewriting_sf_perm h) p with ⟨q, e_q⟩; refine ⟨𝚷 q, by simp[e_q]⟩
 
 @[simp] lemma rew_var_inj_of_inj :
@@ -614,18 +575,15 @@ lemma total_rew_inv :
     simp, split,
     { intros h, funext i, refine (term.rew_var_inj_of_inj I).mp (congr_fun h i) },
     { rintros rfl, simp } }
-| β γ (app p v)   (equal t u) s I := by simp[rew_var]
 | β γ (app r v)   (imply p q) s I := by simp[rew_var]
 | β γ (app r v)   (neg p)     s I := by simp[rew_var]
 | β γ (app r v)   (fal p)     s I := by simp[rew_var, fal_pow]
-| β γ (equal t u) p           s I := by cases p; simp[rew_var, fal_pow, I]
 | β γ (imply p q) r           s I :=
     by cases r; simp[rew_var, fal_pow, @rew_var_inj_of_inj β γ p _ s I, @rew_var_inj_of_inj β γ q _ s I]
 | β γ (neg p)     q           s I :=
     by cases q; simp[rew_var, fal_pow, @rew_var_inj_of_inj β γ p _ s I]
 | β γ (fal p)     verum                   s I := by simp[rew_var]
 | β γ (fal p)     (app r v)   s I := by simp[rew_var]
-| β γ (fal p)     (equal t u) s I := by simp[rew_var]
 | β γ (fal p)     (imply q r) s I := by simp[rew_var]
 | β γ (fal p)     (neg q)     s I := by simp[rew_var]
 | β γ (fal p)     (fal q)     s I := by { simp[rew_var, fal_pow], 
@@ -637,20 +595,23 @@ lemma total_rew_inv :
       { intros h, exact fin.mk.inj_iff.mp (I (congr_arg s (I h)))} },
     simp[this, @rew_var_inj_of_inj _ _ p q _ I'] }
   
-@[simp] lemma pow_inj : ∀ {p q : formula L β} {i : ℕ}, p ↟ i = q ↟ i ↔ p = q :=
-λ p q i, by { simp[pow_eq_rew_var], refine rew_var_inj_of_inj (λ x y, by { simp, exact fin.ext }) }
+@[simp] lemma pow_inj {p q : formula L β} {k : ℕ} : p ↟ k = q ↟ k ↔ p = q :=
+by { simp[pow_eq_rew_var], refine rew_var_inj_of_inj (λ x y, by { simp, exact fin.ext }) }
 
 @[simp] def is_open : Π {β}, formula L β → bool
 | β verum       := tt
 | β (❴p❵ v)     := tt
-| β (equal t u) := tt
 | β (imply p q) := p.is_open && q.is_open
 | β (neg p)     := p.is_open
 | β (fal p)     := ff
 
 @[simp] lemma is_open.verum : (⊤ : formula L β).is_open = tt := rfl
 
-@[simp] lemma is_open.equal (t u : term L β) : (t ≃ u : formula L β).is_open = tt := rfl
+@[simp] lemma is_open.eq [c : has_eq_symbol L] (t u : term L β) : (t ≃ u : formula L β).is_open = tt := rfl
+
+@[simp] lemma is_open.le [c : has_le_symbol L] (t u : term L β) : (t ≼ u : formula L β).is_open = tt := rfl
+
+@[simp] lemma is_open.mem [c : has_mem_symbol L] (t u : term L β) : (t ∊ u : formula L β).is_open = tt := rfl
 
 @[simp] lemma is_open.imply (p q : formula L β) : (p ⟶ q : formula L β).is_open = p.is_open && q.is_open := rfl
 
@@ -665,10 +626,9 @@ lemma total_rew_inv :
 @[simp] def is_open_rew : ∀ {β γ} {p : formula L β} {s : finitary (term L γ) β}, (p.rew s).is_open ↔ p.is_open
 | β γ verum       s := by simp
 | β γ (❴p❵ v)     s := by simp
-| β γ (equal t u) s := by simp
-| β γ (imply p q) s  := by simp[@is_open_rew β γ p s, @is_open_rew β γ q s]
+| β γ (imply p q) s := by simp[@is_open_rew β γ p s, @is_open_rew β γ q s]
 | β γ (neg p)     s := by simp[@is_open_rew β γ p s]
-| β γ (fal p)     s   := by simp
+| β γ (fal p)     s := by simp
 
 @[simp] def is_open_pow : ∀ {p : formula L β} {k : ℕ}, (p ↟ k).is_open ↔ p.is_open :=
 by simp[pow_eq]
@@ -681,5 +641,54 @@ class predicate (L : language.{u}) :=
 (fun_empty : ∀ n, is_empty (L.fn n))
 
 end language
+
+@[reducible] def theory (L : language.{u}) (β) := set (formula L β)
+
+@[reducible] def Theory (L : language.{u}) := Π β, theory L β
+
+namespace theory
+variables {β}
+
+
+
+instance : has_shift (theory L) := ⟨λ β T, (λ p : formula L β, ⤉p) '' T⟩
+
+class proper_theory (T : Theory L) :=
+(proper : ∀ {β} {p : formula L β} (s), p ∈ T β → p.rew s ∈ T β)
+
+end theory
+
+def eq_axiom4 [c:has_eq_symbol L] {n} (f : L.fn n) : formula L 0 :=
+  𝚷* ((⋀ i : fin n, (#⟨i, nat.lt_add_left _ n n i.property⟩ ≃ (#⟨n + i, by simp⟩ : term L (n + n)))) ⟶
+    ((term.app f (λ i, #⟨i, nat.lt_add_left _ n n i.property⟩)) ≃
+      (term.app f (λ i, #⟨n + i, by simp⟩)) : formula L (n + n)))
+
+def eq_axiom5 [c : has_eq_symbol L] {n} (r : L.pr n) : formula L 0 :=
+  𝚷* ((⋀ i : fin n, (#⟨i, nat.lt_add_left _ n n i.property⟩ ≃ (#⟨n + i, by simp⟩ : term L (n + n)))) ⟶
+    ((formula.app r (λ i, #⟨i, nat.lt_add_left _ n n i.property⟩)) ⟶
+      (formula.app r (λ i, #⟨n + i, by simp⟩)) : formula L (n + n)))
+
+inductive provable (T : Theory L) : Π {β}, formula L β → Type u
+| GE : ∀ {β} {p : formula L (β + 1)},
+    provable p → provable (𝚷 p)
+| MP : ∀ {β} {p q : formula L β},
+    provable (p ⟶ q) → provable p → provable q
+| AX : ∀ {β} {p : formula L β},
+    p ∈ T β → provable p
+| p0 : ∀ {β},
+    provable (⊤ : formula L β)
+| p1 : ∀ {β} {p q : formula L β},
+    provable (p ⟶ q ⟶ p)
+| p2 : ∀ {β} {p q r : formula L β},
+    provable ((p ⟶ q ⟶ r) ⟶ (p ⟶ q) ⟶ p ⟶ r)
+| p3 : ∀ {β} {p q : formula L β},
+    provable ((⁻p ⟶ ⁻q) ⟶ q ⟶ p)
+| q1 : ∀ {β} {p : formula L (β + 1)} {t : term L β},
+    provable (𝚷 p ⟶ p.rew (t ::ᶠ ι))
+| q2 : ∀ {β} {p q : formula L (β + 1)},
+    provable (𝚷 (p ⟶ q) ⟶ 𝚷 p ⟶ 𝚷 q)
+| q3 : ∀ {β} {p : formula L β},
+    provable (p ⟶ 𝚷 (⤉p))
+
 
 end fopl
